\item \textbf{Problem 1.3}
For the spin $\frac12$ state $\ket{S_x;+}$ evaluate both sides of the inequality (1.146), that is
$$ \ev{(\Delta A)^2} \ev{(\Delta B)^2} \geq \frac14 |\ev{\comm{A}{B}}|^2$$
for the operators $A = S_x$ and $B = S_y$, and show that the inequality is satisfied. Repeat for the operators $A = S_z$ and $B = S_y$.

\vspace{1cm}
\textbf{Solution}

We start by stating the state $$\ket{S_x;+} = \frac{1}{\sqrt{2}} \qty(\ket + + \ket -)$$ and the operators $S_x,S_y,S_z$ and $S_i^2$
\begin{align*}
	S_x   & = \frac{\hbar}{2} \qty[\op{+}{-} + \ketbra{-}{+}]    \\
	S_y   & = \frac{\hbar}{2} \qty[-i\op{+}{-} + i\ketbra{-}{+}] \\
	S_z   & = \frac{\hbar}{2} \qty[\op{+}{+} - \ketbra{-}]       \\
	S_i^2 & = \frac14 \hbar^2\mathbb{I}
\end{align*}
We now substitute and evaluate the left hand side of the equation (L.H.S.)

\begin{gather*}
	\ev{(\Delta S_x)^2}\ev{(\Delta S_y)^2} \ge \frac{1}{4} | \ev{\comm{S_x}{S_y}} |^2\\
	\ev{(\Delta S_x)^2} = \ev{S_x^2} - \ev{S_x}^2 = \frac{\hbar^2}{4} - \ev{S_x}^2\\
	\ev{S_x} = \ev{S_x}{S_x;+} = \frac{1}{\sqrt{2}} \qty(\bra + + \bra -) \qty[\frac{\hbar}{2} \qty(\op{+}{-} + \ketbra{-}{+})]\frac{1}{\sqrt{2}} \qty(\ket + + \ket -)\\
	= \frac\hbar4 \qty[0 + 0] = 0\\
	\ev{(\Delta S_x)^2} = \frac{\hbar^2}{4}\\
	\intertext{Now for $(\Delta S_y)^2$, we compute $S_y^2$ and $\ev{S_y}$ first}
	S_y^2 = \frac{\hbar^2}{4}\\
	\ev{S_y} = \ev{S_y}{S_x;+} =  \frac{1}{\sqrt{2}} \qty(\bra + + \bra -) \qty[\frac{\hbar}{2} \qty(-i\op{+}{-} + i\ketbra{-}{+})]\frac{1}{\sqrt{2}} \qty(\ket + + \ket -)\\
	\ev{S_y}= \frac{\hbar}{4} \qty[-i+i] = 0 \\
	\ev{(\Delta S_y)^2} = \frac{\hbar^2}{4}\\
	\therefore \ev{(\Delta S_x)^2}\ev{(\Delta S_y)^2} = \frac{\hbar^2}{4}\frac{\hbar^2}{4} = \frac{\hbar^4}{16}
\end{gather*}


Now we evaluate the R.H.S of the equation
\begin{gather*}
	\ev{\comm{S_x}{S_y}} = i\epsilon_{x,y,z} \hbar \ev{S_z} = i\hbar \ev{S_z} = i \hbar \frac{\hbar}{2} \bra{S_x;+}\qty[\op{+}{+} - \ketbra{-}]\ket{S_x;+ }\\
	=i\frac{\hbar^2}{2}  \frac{1}{\sqrt{2}} \qty(\bra + + \bra -) \qty[\op{+}{+} - \ketbra{-}]\frac{1}{\sqrt{2}} \qty(\ket + + \ket -)\\
	= i\frac{\hbar^2}{4} (1 - 1) = 0 \\
	|\ev{\comm{S_x}{S_y}}|^2 = 0
\end{gather*}

So now we have
\[
	\ev{(\Delta S_x)^2}\ev{(\Delta S_y)^2} \ge \frac{1}{4} |\ev{\comm{S_x}{S_y}}|^2 \longrightarrow \frac{\hbar^4}{16} \ge 0
\]

So the relation holds. Now for $A = S_z$ and $B = S_y$. Starting with the L.H.S.

\begin{align*}
	\ev{(\Delta S_z)^2}            & = \ev{S_z^2} - \ev{S_z}^2                        \\
	\ev{(\Delta S_y)^2}            & = \ev{S_y^2} - \ev{S_y}^2                        \\
	\intertext{We already know that $\ev{S_z} = 0$ and we have already stated above $S_i^2 = \frac14 \hbar^2\mathbb{I}$.}
	\ev{S_z^2}                     & = \frac{\hbar^2}{4}                              \\
	\therefore \ev{(\Delta S_z)^2} & = \frac{\hbar^2}{4}                              \\
	\ev{(\Delta S_y)^2}            & = \frac{\hbar^2}{4} \qq{As we have seen before.} \\
\end{align*}
Now we work on the R.H.S.
\begin{gather*}
	\ev{\comm{S_z}{S_y}} = i\epsilon_{z,y,x} \hbar \ev{S_x} = -i\hbar \ev{S_x}= -i \hbar \ev{S_x}{S_x;+}\\
	= -i\hbar\frac{\hbar}{2}\frac12 \bra{S_x;+}\qty(\op{+}{-} + \op{-}{+})\ket{S_x;+ }\\
	= -i\frac{\hbar^2}{2} \frac12  \qty(\bra + + \bra -) \qty[\op{+}{-} + \ketbra{-}{+}] \qty(\ket + + \ket -)\\
	= -i\frac{\hbar^2}{2} \frac12 (\braket{+} \braket{-} + \braket{-} \braket{+}) = -i \frac{\hbar^2}{2} \frac12 (2) = -i\frac{\hbar^2}{2}\\
	|\ev{\comm{S_z}{S_y}}|^2 = \qty(\frac{-i\hbar^2}{2})\qty(\frac{i\hbar^2}{2}) = \frac{\hbar^4}{4}
\end{gather*}


So finally
\[
	\ev{(\Delta S_z)^2}\ev{(\Delta S_y)^2} \ge \frac{1}{4} |\ev{\comm{S_z}{S_y}}|^2 \longrightarrow \frac{\hbar^4}{16} \ge \frac14 \frac{\hbar^4}{4} \longrightarrow \frac{\hbar^4}{16} \ge \frac{\hbar^4}{16}
\]
The relation also holds.
