\item \textbf{Problem 1.6}  Using the rules of bra-ket algebra, prove or evaluate the following: 
\begin{enumerate}
    \item $\Tr(XY) = \Tr(YX)$, where $X$ and $Y$ are operators.
    
    \textbf{Solution:}
    \begin{gather*}
    \Tr(XY) = \sum_{a'} \ev{XY}{a'} = \sum_{b'}\sum_{a'} \mel{a'}{X}{b'} \mel{b'}{Y}{a'} \\
    = \sum_{b'a'} \mel{b'}{Y}{a'} \mel{a'}{X}{b'} = \sum_{b'} \mel{b'}{YX}{b'} = \Tr(YX)
    \end{gather*}
        
    \item $(XY)^\dag = Y^\dagger X^\dag$, where $X$ and $Y$ are operators.
    
    \textbf{Solution:}

    Using two arbitrary kets $\ket \alpha, \ket \beta$
    \begin{gather*}
        \mel{\alpha}{(XY)^\dag}{\beta} = \mel{\beta}{XY}{\alpha}^* = \sum_{a'} \qty(\mel{\beta}{X}{a'}\mel{a'}{Y}{\alpha})^* = \sum_{a'} \mel{a'}{Y}{\alpha}^* \mel{\beta}{X}{a'}^* \\
        = \sum_{a'}\mel{\alpha}{Y^\dag}{a'}\mel{a'}{X^\dag}{\beta} = \mel{\alpha}{Y^\dag X^\dag}{\beta}
    \end{gather*}
    So we have 

    \[
    \mel{\alpha}{(XY)^\dag}{\beta}=\mel{\alpha}{Y^\dag X^\dag}{\beta}
    \]
    for arbitrary $\ket \alpha, \ket \beta$, therefore we must have 
    \[
    (XY)^\dag = Y^\dagger X^\dag
    \]
    
    
    
    \item $\exp[if(A)] =?$ in ket-bra form, where A is a Hermitian operator whose eigenvalues are known.
    
    \textbf{Solution:}
    
    \begin{gather*}
        \exp[if(A)] = \exp[if\qty(\sum_{a'a''} \op{a'} A \op{a''})] \\
        = \exp(if \mqty[\dmat[0]{a',a'' , \ddots}]) = \mqty[\dmat[0]{\exp(if(a')),\exp(if(a'')), \ddots}]\\
        = \sum_{a'}\exp[if(a')]\op{a'}
    \end{gather*}
    
    
    
\end{enumerate}